This problem is about evaluating a diversity index $D$, which is easier to intuit about than the entropy number. This diversity index is supposed to represent a different hypothetical text $T'$ which shares the same entropy $H$ as the origional text $T$. The text $T'$ has all the words appearing in equal frequency $1/D$, so there is $p_i = 1/D$ for $i = 1, ... ,D$. This means that we set $H$ = $H'$, substituting the $p_i$ from $T$ with $p_i' = 1/D$ in $H'$ from $T'$. Also remembering that the sum of the text is from $i=1$ to $D$.

\paragraph{Simpson Concentration}
\[
  S =
  \sum_{i=1}^{n}
  p_i^2
  \addtag
\]

\[
  S = S'
  \addtag
\]

\[
  \sum_{i=1}^{n}
  p_i^2
  =
  \sum_{i=1}^{D}
  (1/D)^2
  \addtag
\]

\[
  \sum_{i=1}^{n}
  p_i^2
  =
  \sum_{i=1}^{D}
  (1/D)^2
  \addtag
\]

\[
  \sum_{i=1}^{n}
  p_i^2
  =
  D
  (1/D)^2
  \addtag
\]

\[
  \sum_{i=1}^{n}
  p_i^2
  =
  (1/D)
  \addtag
\]

\[
  D =
  \left(
    \sum_{i=1}^{n}
    p_i^2
  \right)^{-1}
  \addtag
  =
  S^{-1}
\]

\paragraph{Gini Index}
\[
  G \equiv
  1 - S
  =
  1 -
  \sum_{i=1}^{n}
  p_i^2
  \addtag
\]

\[
  G = G'
  \addtag
\]

\[
  1 -
  \sum_{i=1}^{n}
  p_i^2
  = 
  1 -
  \sum_{i=1}^{n}
  (1/D)^2
  \addtag
\]

\[
  \sum_{i=1}^{n}
  p_i^2
  =
  \sum_{i=1}^{D}
  (1/D)^2
  \addtag
\]

\[
  \sum_{i=1}^{n}
  p_i^2
  =
  D
  (1/D)^2
  \addtag
\]

\[
  \sum_{i=1}^{n}
  p_i^2
  =
  (1/D)
  \addtag
\]

\[
  D =
  \left(
    \sum_{i=1}^{n}
    p_i^2
  \right)^{-1}
  \addtag
  =
  S^{-1}
\]

The diversity index for the Simpson Concentration and the Gini Index come out to be the same!
The diversity index for the Gini Index can even be written in terms of the Simpson Concentration.

\paragraph{Shannon's Entropy}
\[
  H =
  - \sum_{i=1}^{n}
  p_i
  \ln p_i
  \addtag
\]

\[
  H = H'
  \addtag
\]

\[
  H
  =
  - \sum_{i=1}^{D}
  (1/D)
  \ln (1/D)
  \addtag
\]

\[
  H
  =
  - D
  (1/D)
  \ln (1/D)
  \addtag
\]

\[
  H
  =
  - \ln (1/D)
  =
  \ln D
  \addtag
\]

\[
  D
  = 
  e^H
  =
  e^{
    - \sum_{i=1}^{n}
    p_i
    \ln p_i
  }
  \addtag
\]

\paragraph{Renya Entropy, $q \neq 1$}
\[
  H_q^{(R)} =
  \frac{1}{q - 1}
  \left(
    - \ln
    \sum_{i=1}^{n}
      p_i^q
  \right)
  \addtag
\]

\[
  H_q^{(R)} = (H_q^{(R)})'
\]

\[
  \frac{1}{q - 1}
  \left(
    - \ln
    \sum_{i=1}^{n}
      p_i^q
  \right)
  =
  \frac{1}{q - 1}
  \left(
    - \ln
    \sum_{i=1}^{D}
      (1/D)^q
  \right)
  \addtag
\]

\[
  - \ln
  \sum_{i=1}^{n}
    p_i^q
  =
  - \ln
  \sum_{i=1}^{D}
    (1/D)^q
  \addtag
\]

\[
  \sum_{i=1}^{n}
    p_i^q
  =
  \sum_{i=1}^{D}
    (1/D)^q
  \addtag
\]

\[
  \sum_{i=1}^{n}
    p_i^q
  =
  D
  (D)^{-q}
  \addtag
\]

\[
  \sum_{i=1}^{n}
    p_i^q
  =
  D^{q + 1}
  \addtag
\]

\[
  D =
  \left(
  \sum_{i=1}^{n}
    p_i^q
  \right)^{
    \frac{1}{q + 1}
  }
  \addtag
\]

\paragraph{Generalized Tsallis Entropy, $q \neq 1$}
\[
  H_q^{(T)} =
  \frac{1}{q - 1}
  \left(
    1 -
    \sum_{i=1}^{n}
      p_i^q
  \right)
  \addtag
\]

\[
  H_q^{(T)} = (H_q^{(T)})'
\]

\[
  \frac{1}{q - 1}
  \left(
    1 -
    \sum_{i=1}^{n}
      p_i^q
  \right)
  =
  \frac{1}{q - 1}
  \left(
    1 -
    \sum_{i=1}^{D}
      (1/D)^q
  \right)
  \addtag
\]

\[
  1 -
  \sum_{i=1}^{n}
    p_i^q
  =
  1 -
  \sum_{i=1}^{D}
    (1/D)^q
  \addtag
\]

\[
  \sum_{i=1}^{n}
    p_i^q
  =
  \sum_{i=1}^{D}
    (1/D)^q
  \addtag
\]

\[
  \sum_{i=1}^{n}
    p_i^q
  =
  \sum_{i=1}^{D}
    (1/D)^q
  \addtag
\]

\[
  \sum_{i=1}^{n}
    p_i^q
  =
  D
  (D)^{-q}
  \addtag
\]

\[
  \sum_{i=1}^{n}
    p_i^q
  =
  D^{q + 1}
  \addtag
\]

\[
  D =
  \left(
  \sum_{i=1}^{n}
    p_i^q
  \right)^{
    \frac{1}{q + 1}
  }
  \addtag
\]

We see that the Generalized Tallis Entropy and the Renya Entropy come out to be the same!

\paragraph{Matching the Tallis Diversity as $q \to 1$ to Shannon Diversity}

\[
  D_H
  = 
  e^H
  =
  e^{
    - \sum_{i=1}^{n}
    p_i
    \ln p_i
  }
  \addtag
\]

\[
  D_T =
  \left(
  \sum_{i=1}^{n}
    p_i^q
  \right)^{
    \frac{1}{q + 1}
  }
  \addtag
\]

\[
  \lim_{q \to 1} D_T =
  \lim_{q \to 1}
  \left(
  \sum_{i=1}^{n}
    p_i^q
  \right)^{
    \frac{1}{q + 1}
  }
  \addtag
\]

\[
  \lim_{q \to 1} D_T =
  =
  \left(
  \sum_{i=1}^{n}
    p_i
  \right)^{
    1/2
  }
  \addtag
\]

Hmmm, doesn't seem quite right